sha/verif_hmac_init.v
@@ -1,0 +1,1188 @@
+Require Import floyd.proofauto.
+Import ListNotations.
+Require sha.sha.
+Require sha.SHA256.
+Local Open Scope logic.
+
+Require Import sha.spec_sha.
+Require Import sha_lemmas.
+Require Import sha.HMAC_functional_prog.
+
+Require Import sha.hmac091c.
+Require Import HMAC_lemmas.
+Require Import sha.spec_hmac.
+
+Lemma Zlength_max_zero: forall {A:Type} (l:list A), Z.max 0 (Zlength l) = Zlength l.
+Proof. intros.
+       rewrite Z.max_r. trivial.  
+       apply (initial_world.zlength_nonneg _ l).
+Qed.
+
+Definition emptySha:s256state := (nil, (Vundef, (Vundef, (nil, Vundef)))).
+
+Definition postResetHMS key (iS oS: s256state): hmacstate :=
+  (emptySha, (iS, (oS, 
+   (if zlt 64 (Zlength key) then Vint (Int.repr 32) else Vint (Int.repr (Zlength key)), 
+   map Vint (map Int.repr (HMAC_FUN.mkKey key)))))).
+ 
+Definition keyedHMS key: hmacstate :=
+  (emptySha, (emptySha, (emptySha, 
+   (if zlt 64 (Zlength key) then Vint (Int.repr 32) else Vint (Int.repr (Zlength key)), 
+   map Vint (map Int.repr (HMAC_FUN.mkKey key)))))).
+
+Lemma body_hmac_init: semax_body Vprog Gtot 
+       f_HMAC_Init HMAC_Init_spec.
+Proof.
+start_function.
+name ctx' _ctx.
+name key' _key.
+name len' _len.
+simpl_stackframe_of.
+destruct H as [KL1 [KL2 KL3]]. normalize.
+eapply semax_pre with (P':=PROP  (isptr k /\ Forall isbyteZ key /\ isptr c)
+   LOCAL  (`(eq c) (eval_id _ctx); `(eq k) (eval_id _key);
+   `(eq (Vint (Int.repr l))) (eval_id _len);
+   (*`(eq KV) (eval_var sha._K256 (tarray tuint 64))*)
+     (fun rho => (eq KV) (eval_var sha._K256 (tarray tuint 64) (globals_only rho))))
+   SEP 
+   ((EX pad:_, 
+            local (`(eq pad) (eval_var _pad (tarray tuchar 64))) && 
+            `(data_at_ Tsh (tarray tuchar 64) pad));
+   `(data_at_ Tsh t_struct_hmac_ctx_st c); `(data_block Tsh key k);
+   `(K_vector KV))).
+  entailer. apply exp_right with (x:=eval_var _pad (tarray tuchar 64) rho). 
+  entailer. 
+normalize. intros pad. normalize. 
+apply isptrD in H. destruct H as [kb [kofs isptr_k]]; rewrite isptr_k in *.
+apply isptrD in H1. destruct H1 as [cb [cofs isptr_c]]; rewrite isptr_c in *.
+rename H0 into isbyte_key.
+
+(*Sset _reset (Econst_int (Int.repr 0) tint)*)
+forward.
+
+unfold data_block. normalize. 
+
+(*isolate branch if (key != NULL) *)
+apply seq_assoc.
+
+(*given our precondition, we will always have reset=1 after this conditional*)
+remember 
+  (PROP  ()
+   LOCAL  (`(eq (Vint (Int.repr 1))) (eval_id _reset);
+   `(eq pad) (eval_var _pad (tarray tuchar 64));
+   `(eq (Vptr cb cofs)) (eval_id _ctx); `(eq (Vptr kb kofs)) (eval_id _key);
+   `(eq (Vint (Int.repr l))) (eval_id _len);
+   (*`(eq KV) (eval_var sha._K256 (tarray tuint 64))*)
+     (fun rho => (eq KV) (eval_var sha._K256 (tarray tuint 64) (globals_only rho))))
+   SEP  (`(data_at_ Tsh (tarray tuchar 64) pad);
+   `(data_at Tsh t_struct_hmac_ctx_st (keyedHMS key) (Vptr cb cofs));
+   `(array_at tuchar Tsh (tuchars (map Int.repr key)) 0 (Zlength key)
+       (Vptr kb kofs)); `(K_vector KV))) as PostKeyNull. 
+forward_seq. instantiate (1:= PostKeyNull). (*eapply semax_seq.*)
+{ forward_if PostKeyNull.
+  { (* THEN*)
+    simpl. 
+    unfold force_val2, force_val1; simpl. 
+    eapply semax_pre with (P':=
+      (PROP  ()
+       LOCAL 
+         (`(eq (Vint (Int.repr 0))) (eval_id _reset);
+          `(eq pad) (eval_var _pad (tarray tuchar 64)); `(eq c) (eval_id _ctx);
+          `(eq k) (eval_id _key); `(eq (Vint (Int.repr l))) (eval_id _len);
+(*          `(eq KV) (eval_var sha._K256 (tarray tuint 64))*)
+     (fun rho => (eq KV) (eval_var sha._K256 (tarray tuint 64) (globals_only rho))))
+      SEP  (
+          `(data_at_ Tsh (tarray tuchar 64) pad);
+          `(data_at_ Tsh t_struct_hmac_ctx_st (Vptr cb cofs));
+          `(K_vector KV);
+          `(array_at tuchar Tsh (tuchars (map Int.repr key)) 0 (Zlength key) k)))).
+      entailer. simpl. (*unfold typed_true. normalize.*) cancel.
+
+    forward. (*reset =1 *)
+    forward. (*j=HMAC_MAX_MD_CBLOCK*)
+    simpl.
+
+    remember
+     (PROP  ()
+      LOCAL  (
+       `(eq (Vint (Int.repr 1))) (eval_id _reset);
+       `(eq pad) (eval_var _pad (tarray tuchar 64)); `(eq c) (eval_id _ctx);
+       `(eq k) (eval_id _key); `(eq (Vint (Int.repr l))) (eval_id _len);
+       (fun rho => (eq KV) (eval_var sha._K256 (tarray tuint 64) (globals_only rho))))
+(*       `(eq KV) (eval_var sha._K256 (tarray tuint 64)))*)
+      SEP  (`(data_at_ Tsh (tarray tuchar 64) pad);
+            `(data_at Tsh t_struct_hmac_ctx_st (keyedHMS key) (Vptr cb cofs));
+           `(array_at tuchar Tsh (tuchars (map Int.repr key)) 0 (Zlength key)
+             (Vptr kb kofs));
+          `(K_vector KV))) as PostIf_j_Len.
+
+    forward_if PostIf_j_Len. 
+    { (* j < len*)
+      eapply semax_pre with (P':=
+       (PROP  (64 < l)
+        LOCAL 
+         (`(eq (Vint (Int.repr 64))) (eval_id _j);
+          `eq (eval_id _reset) `(Vint (Int.repr 1));
+          `(eq pad) (eval_var _pad (tarray tuchar 64)); `(eq c) (eval_id _ctx);
+          `(eq k) (eval_id _key); `(eq (Vint (Int.repr l))) (eval_id _len);
+(*          `(eq KV) (eval_var sha._K256 (tarray tuint 64))*)
+       (fun rho => (eq KV) (eval_var sha._K256 (tarray tuint 64) (globals_only rho))))
+        SEP  (`(data_at_ Tsh (tarray tuchar 64) pad);
+              `(data_at_ Tsh t_struct_hmac_ctx_st c);
+              `(K_vector KV);
+              `(array_at tuchar Tsh (tuchars (map Int.repr key)) 0 (Zlength key) k)))).
+        entailer. 
+      normalize. rename H into lt_64_l. 
+
+      (*call to SHA256_init*)
+      eapply semax_seq'.
+      frame_SEP 1.
+      unfold data_at_.
+      unfold_data_at 1%nat.
+      rewrite (field_at_data_at Tsh t_struct_hmac_ctx_st [_md_ctx]); try reflexivity.
+      normalize. 
+      rename H into SCc. rename H0 into ACc.
+      rewrite isptr_c; simpl.
+      (*rewrite at_offset'_eq.
+      2: rewrite isptr_c; simpl; rewrite Int.add_zero; reflexivity.*)
+      forward_call (Vptr cb cofs). 
+      { assert (FR: Frame = [
+        `(field_at Tsh t_struct_hmac_ctx_st [_key_length] Vundef (Vptr cb cofs));
+        `(field_at Tsh t_struct_hmac_ctx_st [_key] [] (Vptr cb cofs));
+        `(field_at Tsh t_struct_hmac_ctx_st [_o_ctx]
+               ([], (Vundef, (Vundef, ([], Vundef)))) (Vptr cb cofs));
+        `(field_at Tsh t_struct_hmac_ctx_st [_i_ctx]
+             ([], (Vundef, (Vundef, ([], Vundef)))) (Vptr cb cofs))]).
+         subst Frame. reflexivity.
+       rewrite FR. clear FR Frame.   
+       entailer. cancel. 
+      } 
+      after_call. rewrite isptr_c; simpl. 
+      normalize.
+
+      (*call to SHA256_Update*)
+      erewrite (split_offset_array_at _ _ _ 0 l); try reflexivity. 2: subst l; omega.
+      normalize.
+      rewrite isptr_k in H, H0. simpl in H, H0. rewrite Zplus_0_r in H.
+      rename H into OIR_kofs. rename H0 into OIR_kofs_key.
+      eapply semax_seq'.
+      frame_SEP 8 0 2.
+      remember (init_s256abs, key, Vptr cb cofs,
+                Vptr kb kofs, Tsh, l, KV) as WITNESS.
+      forward_call WITNESS.
+      { assert (FR: Frame = []).
+          subst Frame. reflexivity.
+        rewrite FR. clear FR Frame.   
+        subst WITNESS. entailer.
+        apply andp_right.
+           apply prop_right. 
+             rewrite int_max_signed_eq in KL2. 
+             rewrite int_max_unsigned_eq; omega.
+        cancel. unfold data_block. 
+          simpl. (*not doing this simpl results in a coq anomaly in entailer, and and_pright is not applicable*)
+          apply andp_right. entailer. cancel. 
+      } 
+      after_call. subst WITNESS. simpl. intros rho. normalize. simpl.
+
+     (*commute fun a => and EX x*)
+     apply semax_pre with (P':=
+      EX  xx : s256abs,
+  (PROP  ()
+   LOCAL  (tc_environ Delta; tc_environ Delta;
+   `(eq (Vint (Int.repr 1))) (eval_id _reset);
+   `(eq pad) (eval_var _pad (tarray tuchar 64));
+   `(eq (Vptr cb cofs)) (eval_id _ctx); `(eq k) (eval_id _key);
+   `(eq (Vint (Int.repr l))) (eval_id _len);
+(*   `(eq KV) (eval_var sha._K256 (tarray tuint 64))*)
+       (fun rho => (eq KV) (eval_var sha._K256 (tarray tuint 64) (globals_only rho))))
+   SEP 
+   (`(fun a : environ =>
+      (PROP  (update_abs (firstn (Z.to_nat l) key) init_s256abs xx)
+       LOCAL ()
+       SEP  (`(K_vector KV); `(sha256state_ xx (Vptr cb cofs));
+       `(data_block Tsh key (Vptr kb kofs)))) a) globals_only;
+   `(array_at tuchar Tsh (fun i : Z => tuchars (map Int.repr key) (i + l)) 0
+       (Zlength key - l) (offset_val (Int.repr l) k));
+   `(field_at Tsh t_struct_hmac_ctx_st [_key_length] Vundef (Vptr cb cofs));
+   `(field_at Tsh t_struct_hmac_ctx_st [_key] [] (Vptr cb cofs));
+   `(field_at Tsh t_struct_hmac_ctx_st [_o_ctx]
+       ([], (Vundef, (Vundef, ([], Vundef)))) (Vptr cb cofs));
+   `(field_at Tsh t_struct_hmac_ctx_st [_i_ctx]
+       ([], (Vundef, (Vundef, ([], Vundef)))) (Vptr cb cofs));
+   `(data_at_ Tsh (tarray tuchar 64) pad)))).
+       entailer. clear x x0 x1. rename x2 into a. apply exp_right with (x:=a).
+       entailer.
+   apply extract_exists_pre. intros ctxSha. simpl. normalize. simpl.
+
+   (*call Final*)
+   rewrite (field_at_data_at Tsh t_struct_hmac_ctx_st [_key]); try reflexivity.
+   normalize. 
+   rewrite at_offset'_eq.
+     2: simpl; rewrite Int.add_zero; reflexivity.
+   unfold nested_field_offset2, nested_field_type2; simpl.
+   unfold tarray.
+   erewrite (data_at_array_at Tsh tuchar 64 noattr []).
+     2: apply JMeq.JMeq_refl. 
+     2: omega.
+     2: reflexivity. 
+   erewrite (split_offset_array_at _ _ _ 0 32 64); try reflexivity. 2: omega.
+   normalize.
+   eapply semax_seq'.
+   frame_SEP 2 3 0.
+   remember (ctxSha, Vptr cb (Int.add cofs (Int.repr 328)),
+             Vptr cb cofs, Tsh, Tsh, KV) as WITNESS.
+   forward_call WITNESS.
+     { assert (FR: Frame = []).
+         subst Frame. reflexivity.
+       rewrite FR. clear FR Frame.   
+       subst WITNESS. entailer. cancel.
+       rewrite memory_block_array_tuchar'. cancel. trivial. omega.
+     }
+     after_call. subst WITNESS. simpl. intros rho. normalize. simpl. normalize. simpl.
+
+   (*call memset*)
+   (* doing this: eapply semax_seq'. frame_SEP 3. requires us to do the swap fun a=> vs EX
+      after the call, which leaves a state that still doesn't nicely normalize *)
+   remember (Tsh, Vptr cb (Int.add cofs (Int.repr 360)), 32, Int.zero) as WITNESS.
+   forward_call WITNESS.
+     { assert (FR: Frame = [`(K_vector KV);
+         `(data_at_ Tsh sha.t_struct_SHA256state_st (Vptr cb cofs));
+         `(data_block Tsh (sha_finish ctxSha) (Vptr cb (Int.add cofs (Int.repr 328))));
+         `(data_block Tsh key (Vptr kb kofs));
+         `(array_at tuchar Tsh (fun i : Z => tuchars (map Int.repr key) (i + l)) 0
+              (Zlength key - l) (offset_val (Int.repr l) k));
+         `(field_at Tsh t_struct_hmac_ctx_st [_key_length] Vundef (Vptr cb cofs));
+         `(field_at Tsh t_struct_hmac_ctx_st [_o_ctx]
+              ([], (Vundef, (Vundef, ([], Vundef)))) (Vptr cb cofs));
+         `(field_at Tsh t_struct_hmac_ctx_st [_i_ctx]
+              ([], (Vundef, (Vundef, ([], Vundef)))) (Vptr cb cofs));
+(*         `(data_at_ Tsh t_struct_SHA256state_st sha);*)
+         `(data_at_ Tsh (Tarray tuchar 64 noattr) pad)]).
+         subst Frame. reflexivity.
+       rewrite FR. clear FR Frame.   
+       entailer. cancel. 
+       rewrite memory_block_array_tuchar'. cancel. trivial. omega.
+     } 
+     after_call. subst WITNESS. normalize. subst retval0. 
+  clear x.
+   (*swap fun a=> with EX
+   apply semax_pre with (P':=
+    EX  x : val,
+  (PROP  ()
+   LOCAL  (tc_environ Delta; tc_environ Delta; tc_environ Delta;
+   tc_environ Delta; `(eq (Vint (Int.repr 1))) (eval_id _reset);
+   `(eq sha) (eval_var _sha_ctx t_struct_SHA256state_st);
+   `(eq pad) (eval_var _pad (Tarray tuchar 64 noattr));
+   `(eq (Vptr cb cofs)) (eval_id _ctx); `(eq k) (eval_id _key);
+   `(eq (Vint (Int.repr l))) (eval_id _len);
+   `(eq KV) (eval_var sha._K256 (Tarray tuint 64 noattr)))
+   SEP 
+   (fun a : environ =>
+    `(fun x0 : environ =>
+      local (`(eq (Vptr cb (Int.add cofs (Int.repr 360)))) retval) x0 &&
+      `(array_at tuchar Tsh (fun _ : Z => Vint Int.zero) 0 32
+          (Vptr cb (Int.add cofs (Int.repr 360)))) x0)
+      (fun rho : environ => env_set (globals_only rho) ret_temp x) a;
+   `(K_vector KV);
+   `(data_at_ Tsh sha.t_struct_SHA256state_st (Vptr cb cofs));
+   `(data_block Tsh (sha_finish mdSha)
+       (Vptr cb (Int.add cofs (Int.repr 328))));
+   `(data_block Tsh key (Vptr kb kofs));
+   `(array_at tuchar Tsh (fun i : Z => tuchars (map Int.repr key) (i + l)) 0
+       (Zlength key - l) (offset_val (Int.repr l) k));
+   `(field_at Tsh t_struct_hmac_ctx_st [_key_length] Vundef (Vptr cb cofs));
+   `(field_at Tsh t_struct_hmac_ctx_st [_o_ctx]
+       ([], (Vundef, (Vundef, ([], Vundef)))) (Vptr cb cofs));
+   `(field_at Tsh t_struct_hmac_ctx_st [_i_ctx]
+       ([], (Vundef, (Vundef, ([], Vundef)))) (Vptr cb cofs));
+   `(data_at_ Tsh t_struct_SHA256state_st sha);
+   `(data_at_ Tsh (Tarray tuchar 64 noattr) pad)))).
+    entailer.
+    apply exp_right with (x:=Vptr cb (Int.add cofs (Int.repr 360))).
+    entailer.
+   apply extract_exists_pre. intros x. simpl. normalize.
+     unfold local. simpl. red. normalize.*)
+
+   forward. (*ctx->key_length=32*)
+
+   subst PostIf_j_Len.
+   entailer. 
+   cancel.
+   unfold data_block. entailer. cancel. 
+   unfold data_at_.
+   destruct (zlt 64 (Zlength key)). 2: omega.
+   unfold_data_at 2%nat.
+   cancel. 
+   rewrite (field_at_data_at Tsh t_struct_hmac_ctx_st [_key]); try reflexivity.
+     entailer.
+     rewrite at_offset'_eq.
+     2: simpl; rewrite Int.add_zero; reflexivity.
+     unfold nested_field_offset2, nested_field_type2; simpl.
+     unfold tarray.
+     erewrite (data_at_array_at Tsh tuchar 64 noattr).
+     2: apply JMeq.JMeq_refl. 
+     2: omega.
+     2: reflexivity. 
+     erewrite (split_offset_array_at _ _ _ 0 32 64); try reflexivity. 2: omega.
+     entailer. unfold offset_val. rewrite Int.add_assoc.
+        assert (I360: Int.add (Int.repr 328) (Int.repr 32) = Int.repr 360).
+          reflexivity. 
+        rewrite I360; clear I360.  simpl.
+     assert (LengthShaFinish: Zlength (sha_finish ctxSha) = 32).
+                 unfold sha_finish. destruct ctxSha.
+        rewrite <- functional_prog.SHA_256'_eq, Zlength_correct, length_SHA256'. reflexivity.
+     rewrite array_at_ext with (f':= fun i : Z =>
+         ZnthV tuchar (map Vint (map Int.repr (HMAC_FUN.mkKey key))) (i + 32)).
+     Focus 2. intros. unfold ZnthV. if_tac. omega.
+              assert (Z32: (Z.to_nat i < 32)%nat).
+                  clear - H5; destruct H5 as [XX YY]. rewrite Z2Nat.inj_lt in YY.
+                  apply YY. omega. omega.
+               unfold HMAC_FUN.mkKey. simpl.
+               assert (Kgt: Zlength key > 64) by omega.
+               apply Zgt_is_gt_bool in Kgt.
+               rewrite Kgt. unfold HMAC_FUN.zeroPad. repeat rewrite map_app.
+               rewrite app_nth2; repeat rewrite map_length; rewrite length_SHA256'.
+                 remember (Nlist 0 (SHA256_BlockSize - Z.to_nat SHA256_DIGEST_LENGTH)) as NL.
+                 simpl.
+                 assert (I: (Z.to_nat (i + 32) - 32)%nat = Z.to_nat i).
+                             destruct H5. specialize (Z2Nat.inj_sub (i+32) 32).
+                             simpl; intros HH. rewrite <- HH, Zplus_comm, Zminus_plus. trivial.
+                             omega. 
+                 rewrite I. subst NL. 
+                 assert (SHA32: (SHA256_BlockSize - Z.to_nat SHA256_DIGEST_LENGTH)%nat = 32%nat) by reflexivity.
+                 rewrite SHA32.
+                 rewrite nth_map' with (d':=Int.zero).
+                   rewrite nth_map' with (d':=Z0).
+                     rewrite nth_Nlist; trivial.
+                     rewrite length_Nlist; trivial.
+                   rewrite  map_length, length_Nlist; trivial.
+                 apply (Z2Nat.inj_le 32 (i + 32)); omega.
+
+     cancel.
+     rewrite LengthShaFinish.
+     rewrite array_at_ext with (f':=ZnthV tuchar (map Vint (map Int.repr (HMAC_FUN.mkKey key)))).
+     Focus 2. unfold tuchars, sha_finish; intros. destruct ctxSha. simpl.
+              assert (Z32: (Z.to_nat i < 32)%nat).
+                  clear - H5; destruct H5 as [XX YY]. rewrite Z2Nat.inj_lt in YY.
+                  apply YY. omega. omega.    
+              unfold ZnthV. destruct (zlt i 0). omega.   
+              rewrite nth_map' with (d':=Int.zero). rewrite nth_map' with (d':=Z0). 
+              rewrite nth_map' with (d':=Int.zero). rewrite nth_map' with (d':=Z0). 
+              f_equal. f_equal. unfold HMAC_FUN.mkKey. simpl. 
+              assert (Z6: Zlength key > 64) by omega. 
+              apply Zgt_is_gt_bool in Z6; rewrite Z6.
+              unfold HMAC_FUN.zeroPad.
+              rewrite <- functional_prog.SHA_256'_eq.
+              rewrite app_nth1. inversion H. subst. clear H. simpl in *.
+                      rewrite <- H17. rewrite firstn_precise. trivial.
+                      rewrite Zlength_correct, Nat2Z.id; trivial.
+              rewrite length_SHA256'; trivial.
+              rewrite HMAC_FUN.mkKey_length; unfold SHA256_BlockSize; simpl. omega.
+              rewrite map_length, HMAC_FUN.mkKey_length; unfold SHA256_BlockSize; simpl. omega.
+              rewrite <- functional_prog.SHA_256'_eq, length_SHA256'. trivial.
+              rewrite map_length, <- functional_prog.SHA_256'_eq, length_SHA256'. trivial. 
+     cancel.
+   rewrite (field_at_data_at Tsh t_struct_hmac_ctx_st [_md_ctx]); try reflexivity.
+     normalize. 
+     rewrite at_offset'_eq.
+     2: simpl; rewrite Int.add_zero; reflexivity.
+     unfold nested_field_offset2, nested_field_type2; simpl. rewrite Int.add_zero.
+     cancel. rewrite <- Zminus_diag_reverse. rewrite array_at_emp. normalize.
+     destruct (zlt 64 (Zlength key)). trivial. omega.
+   } 
+
+   { (* j >= len*)
+     eapply semax_pre with (P':=
+       (PROP  (64 >= l)
+        LOCAL 
+         (`(eq (Vint (Int.repr 64))) (eval_id _j);
+          `eq (eval_id _reset) `(Vint (Int.repr 1));
+          `(eq pad) (eval_var _pad (tarray tuchar 64)); `(eq c) (eval_id _ctx);
+          `(eq k) (eval_id _key); `(eq (Vint (Int.repr l))) (eval_id _len);
+(*          `(eq KV) (eval_var sha._K256 (tarray tuint 64))*)
+       (fun rho => (eq KV) (eval_var sha._K256 (tarray tuint 64) (globals_only rho))))
+        SEP  (`(data_at_ Tsh (tarray tuchar 64) pad);
+              (*`(data_at_ Tsh t_struct_hmac_ctx_st c);*)
+              `(data_at Tsh t_struct_hmac_ctx_st (default_val t_struct_hmac_ctx_st) c);
+              `(K_vector KV);
+              `(array_at tuchar Tsh (tuchars (map Int.repr key)) 0 (Zlength key) k)))).
+        entailer. 
+     normalize. rename H into ge_64_l. clear x0 x1 x. 
+
+     (*call to memcpy*)
+     (*eapply semax_seq'.*)
+     focus_SEP 1 3.
+     (*unfold data_at_. *)
+     unfold_data_at 1%nat.
+     rewrite (field_at_data_at Tsh t_struct_hmac_ctx_st [_key]); try reflexivity.
+     normalize. 
+     rename H into SCc. rename H0 into ACc.
+     rewrite isptr_c; simpl.
+     rewrite at_offset_data_at. unfold nested_field_type2, nested_field_offset2; simpl.
+     unfold tarray.
+     erewrite data_at_array_at. 2: apply JMeq.JMeq_refl. 2: omega. 2: reflexivity.
+     erewrite (split_offset_array_at _ _ _ 0 l 64); try reflexivity. 2: omega.
+     normalize.
+     rename H into OIR0_328. rename H0 into OIR64_328.
+
+     unfold tuchars. remember (64 - l) as l64.
+     remember ((Tsh, Tsh), Vptr cb (Int.add cofs (Int.repr 328)), 
+             k, mkTrep (Tarray tuchar (Zlength key) noattr) 
+                     (map Vint (map Int.repr key))) as WITNESS.
+     forward_call WITNESS.
+     { assert (FR: Frame = [
+        `(array_at tuchar Tsh (fun i : Z => ZnthV tuchar [] (i + l)) 0 l64
+            (offset_val (Int.repr l) (Vptr cb (Int.add cofs (Int.repr 328)))));
+        `(field_at Tsh t_struct_hmac_ctx_st [_key_length] Vundef (Vptr cb cofs));
+        `(field_at Tsh t_struct_hmac_ctx_st [_o_ctx]
+            ([], (Vundef, (Vundef, ([], Vundef)))) (Vptr cb cofs));
+        `(field_at Tsh t_struct_hmac_ctx_st [_i_ctx]
+            ([], (Vundef, (Vundef, ([], Vundef)))) (Vptr cb cofs));
+        `(field_at Tsh t_struct_hmac_ctx_st [_md_ctx]
+            ([], (Vundef, (Vundef, ([], Vundef)))) (Vptr cb cofs));
+        `(data_at_ Tsh (Tarray tuchar 64 noattr) pad);
+        (*`(array_at tuchar Tsh (ZnthV tuchar []) 0 64 pad);*)
+        `(K_vector KV)]).
+         subst Frame. reflexivity.
+       rewrite FR. clear FR Frame.   
+       subst WITNESS. entailer.
+         rewrite Zlength_max_zero.
+         assert ( match Zlength key with
+                     | 0 => 0
+                     | Z.pos y' => Z.pos y'
+                     | Z.neg y' => Z.neg y'
+                 end = Zlength key).
+            destruct (Zlength key); reflexivity.
+       rewrite H0; clear H0.  
+       apply andp_right.
+         apply prop_right. split. omega. split; trivial.
+          rewrite int_max_unsigned_eq.
+         rewrite int_max_signed_eq in KL2; omega. 
+       cancel.
+       rewrite sepcon_comm.
+       apply sepcon_derives.
+         erewrite data_at_array_at.
+         apply array_lemmas.array_at_ext'. intros. reflexivity. 
+         trivial. omega. reflexivity. (*  unfold cVint, ZnthV; intros.
+         if_tac. omega. 
+              rewrite nth_map' with (d':=Int.zero). trivial.
+              rewrite map_length. clear - H0.
+              rewrite Zlength_correct in H0; destruct H0 as [XX YY].
+              apply Z2Nat.inj_lt in YY; trivial. rewrite Nat2Z.id in YY; trivial. omega.*)
+       rewrite memory_block_array_tuchar'. cancel.
+         reflexivity. omega.
+     } 
+     after_call. subst WITNESS. normalize. simpl. subst retval0. 
+       remember (map Vint (map Int.repr key)) as CONT.
+
+   (*call memset*)
+   remember (Tsh, Vptr cb (Int.add cofs (Int.repr (Zlength key + 328))), l64, Int.zero) as WITNESS.
+   forward_call WITNESS.
+     { assert (FR: Frame = [
+        `(data_at Tsh (Tarray tuchar (Zlength key) noattr)
+              CONT (Vptr cb (Int.add cofs (Int.repr 328))));
+        `(data_at Tsh (Tarray tuchar (Zlength key) noattr)
+              CONT k);
+         (* `(array_at tuchar Tsh CONT 0 l k);
+         `(array_at tuchar Tsh CONT 0 l (Vptr cb (Int.add cofs (Int.repr 328))));*)
+         `(field_at Tsh t_struct_hmac_ctx_st [_key_length] Vundef (Vptr cb cofs));
+         `(field_at Tsh t_struct_hmac_ctx_st [_o_ctx]
+             ([], (Vundef, (Vundef, ([], Vundef)))) (Vptr cb cofs));
+         `(field_at Tsh t_struct_hmac_ctx_st [_i_ctx]
+             ([], (Vundef, (Vundef, ([], Vundef)))) (Vptr cb cofs));
+         `(field_at Tsh t_struct_hmac_ctx_st [_md_ctx]
+             ([], (Vundef, (Vundef, ([], Vundef)))) (Vptr cb cofs));
+         `(data_at_ Tsh (Tarray tuchar 64 noattr) pad);
+         (*`(array_at tuchar Tsh (ZnthV tuchar []) 0 64 pad);*)
+         `(K_vector KV)]).
+         subst Frame. reflexivity.
+       rewrite FR. clear FR Frame.   
+       subst WITNESS. entailer.
+       apply andp_right. apply prop_right.
+         clear - KL2; split.
+           specialize (initial_world.zlength_nonneg _ key); intros.
+           rewrite int_max_unsigned_eq. omega.
+         unfold offset_val. rewrite Zplus_comm. trivial.
+       cancel. rewrite Zplus_comm.
+       rewrite memory_block_array_tuchar'. cancel. trivial. omega.
+     } 
+     after_call. subst WITNESS. normalize. subst retval0. 
+
+   forward. (*ctx->key_length=len*)
+
+   subst PostIf_j_Len. entailer. cancel.
+   unfold_data_at 3%nat. entailer.
+   cancel.
+   destruct (zlt 64 (Zlength key)). omega. cancel.  
+   apply sepcon_derives.
+   Focus 2. 
+      erewrite data_at_array_at. unfold tuchars. apply derives_refl.
+      reflexivity. omega. reflexivity.
+  (*
+   unfold_data_at 1%nat.
+   cancel.*)
+   rewrite (field_at_data_at Tsh t_struct_hmac_ctx_st [_key]); try reflexivity.
+     entailer.
+     rewrite at_offset'_eq.
+     2: simpl; rewrite Int.add_zero; reflexivity.
+     remember (64 - Zlength key) as ZK64. 
+     unfold nested_field_offset2, nested_field_type2; simpl.
+     unfold tarray.
+     erewrite (data_at_array_at Tsh tuchar 64 noattr).
+     2: apply JMeq.JMeq_refl. 
+     2: omega.
+     2: reflexivity. 
+     erewrite (split_offset_array_at _ _ _ 0 (Zlength key) 64); try reflexivity. 2: omega.
+     entailer. unfold offset_val. rewrite Int.add_assoc. rewrite add_repr. rewrite (Zplus_comm 328).
+     rewrite sepcon_comm. 
+     assert (F64: false = (Zlength key >? 64)). 
+       rewrite Z.gtb_ltb. symmetry. apply Fcore_Zaux.Zlt_bool_false. omega.
+     apply sepcon_derives. 
+       erewrite data_at_array_at. 2: apply JMeq.JMeq_refl. 2: omega. 2: reflexivity.
+       apply array_lemmas.array_at_ext'.
+         unfold tuchars, cVint, ZnthV; intros. if_tac. omega.
+         assert (Z32: (Z.to_nat i < length key)%nat).
+                  clear - H0; destruct H0 as [XX YY]. rewrite Zlength_correct, Z2Nat.inj_lt in YY.
+                  rewrite Nat2Z.id in YY; trivial. trivial. omega. 
+         apply eq_sym.
+         assert (L1: (Z.to_nat i < length (HMAC_FUN.mkKey key))%nat).
+           rewrite HMAC_FUN.mkKey_length; unfold SHA256_BlockSize.
+           assert (Zlength key <= 64) by omega.  apply Z2Nat.inj_le in H3. simpl in H3.
+           rewrite Zlength_correct, Nat2Z.id in H3. omega.
+           omega. omega.
+         rewrite nth_map' with (d':=Int.zero).
+         rewrite nth_map' with (d':=Int.zero).
+         rewrite nth_map' with (d':=Z0); trivial.
+         rewrite nth_map' with (d':=Z0); trivial. f_equal. f_equal.         
+         eapply mkKey_left; trivial. 
+         rewrite map_length; trivial. rewrite map_length; trivial. 
+       apply array_lemmas.array_at_ext'.
+         unfold tuchars, cVint, ZnthV; intros. if_tac. omega.
+         assert (L1: (Z.to_nat (i + Zlength key) < length (HMAC_FUN.mkKey key))%nat).
+           rewrite HMAC_FUN.mkKey_length; unfold SHA256_BlockSize.
+           destruct H0. 
+           apply (Z2Nat.inj_lt (i+ Zlength key) 64). omega. omega. omega.
+         rewrite nth_map' with (d':=Int.zero).
+         rewrite nth_map' with (d':=Z0). f_equal.
+         rewrite (mkKey_right _ F64 (i + Zlength key)); trivial. omega. trivial.
+         rewrite map_length; trivial.
+  }
+
+  intros. entailer. unfold POSTCONDITION, abbreviate; simpl. entailer.
+
+  }
+  { (*key == NULL*)
+     forward.
+     entailer.
+  }
+  { (*side condition of forward_if key != NULL*)
+    intros. entailer. unfold overridePost, normal_ret_assert; simpl. 
+    if_tac. simpl. entailer. simpl. entailer.
+  }
+}
+
+(*isolate branch if (reset) *)
+apply seq_assoc.
+
+remember (EX iSA:_, EX iS:_, EX oSA:_, EX oS:_,
+          PROP  (innerShaInit (map Byte.repr (HMAC_FUN.mkKey key)) iSA /\ s256_relate iSA iS /\
+                 outerShaInit (map Byte.repr (HMAC_FUN.mkKey key)) oSA /\ s256_relate oSA oS)
+                 LOCAL  (
+                 `(eq pad) (eval_var _pad (tarray tuchar 64));
+                 `(eq (Vptr cb cofs)) (eval_id _ctx);
+                 `(eq (Vptr kb kofs)) (eval_id _key);
+                 `(eq (Vint (Int.repr l))) (eval_id _len);
+   (*`(eq KV) (eval_var sha._K256 (tarray tuint 64))*)
+     (fun rho => (eq KV) (eval_var sha._K256 (tarray tuint 64) (globals_only rho))))
+
+                 SEP  (
+                 `(array_at_ tuchar Tsh 0 64 pad);
+                 `(data_at Tsh t_struct_hmac_ctx_st (postResetHMS key iS oS)
+                     (Vptr cb cofs));
+                 `(array_at tuchar Tsh (tuchars (map Int.repr key)) 0
+                     (Zlength key) (Vptr kb kofs)); `(K_vector KV)))
+  as PostResetBranch.
+(*forward_seq. instantiate (1:= PostResetBranch).*)
+subst PostKeyNull.
+eapply semax_seq. instantiate (1:=PostResetBranch).
+{ forward_if PostResetBranch. 
+  { (* THEN*)
+    remember (cVint (force_int oo ZnthV tuchar (map Vint (map Int.repr 
+              (map Byte.unsigned (HMAC_FUN.mkArg (map Byte.repr (HMAC_FUN.mkKey key)) Ipad)))))) as IPADcont.
+    remember (cVint (force_int oo ZnthV tuchar (map Vint (map Int.repr 
+              (map Byte.unsigned (HMAC_FUN.mkArg (map Byte.repr (HMAC_FUN.mkKey key)) Opad)))))) as OPADcont.
+    assert (ZLI: Zlength (HMAC_FUN.mkArgZ (map Byte.repr (HMAC_FUN.mkKey key)) Ipad) = 64).
+            rewrite Zlength_mkArgZ.
+            repeat rewrite map_length. rewrite HMAC_FUN.mkKey_length.
+            unfold SHA256_BlockSize; simpl. trivial. 
+    assert (ZLO: Zlength (HMAC_FUN.mkArgZ (map Byte.repr (HMAC_FUN.mkKey key)) Opad) = 64).
+            rewrite Zlength_mkArgZ.
+            repeat rewrite map_length. rewrite HMAC_FUN.mkKey_length.
+            unfold SHA256_BlockSize; simpl. trivial. 
+    remember (ZnthV tuchar (default_val (Tarray tuchar 64 noattr))) as DEFAULTcont.
+    unfold data_at_, tuchars, tarray.
+    erewrite data_at_array_at; try reflexivity. 2: omega.
+    rewrite array_at_isptr. normalize. apply isptrD in H. destruct H as [pb [pofs Hpad]]. subst pad.
+    forward_seq. 
+    instantiate (1:= 
+      (PROP  ()
+       LOCAL  (`(typed_true (typeof (Etempvar _reset tint)))
+                 (eval_expr (Etempvar _reset tint));
+        `(eq (Vint (Int.repr 1))) (eval_id _reset);
+        `(eq (Vptr pb pofs)) (eval_var _pad (Tarray tuchar 64 noattr));
+        `(eq (Vptr cb cofs)) (eval_id _ctx); `(eq (Vptr kb kofs)) (eval_id _key);
+        `(eq (Vint (Int.repr l))) (eval_id _len);
+    (*`(eq KV) (eval_var sha._K256 (tarray tuint 64))*)
+        (fun rho => (eq KV) (eval_var sha._K256 (tarray tuint 64) (globals_only rho))))
+       SEP 
+        (`(array_at tuchar Tsh IPADcont 0 64 (Vptr pb pofs));
+         `(data_at Tsh t_struct_hmac_ctx_st (keyedHMS key) (Vptr cb cofs));
+         `(array_at tuchar Tsh (tuchars (map Int.repr key)) 0 (Zlength key) (Vptr kb kofs));
+        `(K_vector KV)))).
+    { (*ipad loop*)
+      forward_for_simple_bound' 64 (EX i:Z, 
+        (PROP  ()
+         LOCAL  (`(typed_true (typeof (Etempvar _reset tint)))
+                     (eval_expr (Etempvar _reset tint));
+                 `(eq (Vint (Int.repr 1))) (eval_id _reset);
+                 `(eq (Vptr pb pofs)) (eval_var _pad (tarray tuchar 64));
+                 `(eq (Vptr cb cofs)) (eval_id _ctx);
+                 `(eq (Vptr kb kofs)) (eval_id _key);
+                 `(eq (Vint (Int.repr l))) (eval_id _len);
+    (*`(eq KV) (eval_var sha._K256 (tarray tuint 64))*)
+        (fun rho => (eq KV) (eval_var sha._K256 (tarray tuint 64) (globals_only rho))))
+         SEP  (
+          `(array_at tuchar Tsh IPADcont 0 i (Vptr pb pofs));
+          `(array_at tuchar Tsh DEFAULTcont i 64 (Vptr pb pofs));
+          `(data_at Tsh t_struct_hmac_ctx_st (keyedHMS key) (Vptr cb cofs));
+          `(array_at tuchar Tsh (ZnthV tuchar (map Vint (map Int.repr key))) 0
+               (Zlength key) (Vptr kb kofs)); `(K_vector KV)))).
+      { admit. (*K256 closed*) }
+      { (*precondition implies "invariant"*) 
+        rewrite array_at_emp. normalize. entailer.
+        unfold array_at. normalize. destruct H4. abstract entailer.
+      }
+      { unfold normal_ret_assert. simpl. intros rho. 
+        rewrite array_at_emp. entailer.
+      }
+      { unfold_data_at 1%nat. normalize.
+        rewrite (field_at_data_at Tsh t_struct_hmac_ctx_st [_key]); try reflexivity.
+        normalize. rename H into I. rename H0 into SCc. rename H1 into ACc.
+        rewrite at_offset'_eq.
+        2: simpl; rewrite Int.add_zero; reflexivity.
+        eapply semax_pre0; [ apply now_later | ].
+        eapply semax_post_flipped'.
+        { subst PostResetBranch.
+          eapply NEWsemax_loadstore_array
+          with (P:= nil)
+          (Q:= [`(eq (Vint (Int.repr i))) (eval_id _i);
+            `(eq (Vint (Int.repr 64))) (eval_expr (Econst_int (Int.repr 64) tint));
+            `(typed_true tint) (eval_expr (Etempvar _reset tint));
+            `(eq (Vint (Int.repr 1))) (eval_id _reset);
+            `(eq (Vptr pb pofs)) (eval_var _pad (tarray tuchar 64));
+            `(eq (Vptr cb cofs)) (eval_id _ctx);
+            `(eq (Vptr kb kofs)) (eval_id _key);
+            `(eq (Vint (Int.repr l))) (eval_id _len);
+   (*`(eq KV) (eval_var sha._K256 (tarray tuint 64))*)
+     (fun rho => (eq KV) (eval_var sha._K256 (tarray tuint 64) (globals_only rho)))])
+          (R:= [`(field_at Tsh t_struct_hmac_ctx_st [_key_length]
+               (if zlt 64 (Zlength key)
+                then Vint (Int.repr 32)
+                else Vint (Int.repr (Zlength key))) (Vptr cb cofs));
+            `(data_at Tsh (nested_field_type2 t_struct_hmac_ctx_st [_key])
+                (map Vint (map Int.repr (HMAC_FUN.mkKey key)))
+               (offset_val
+                 (Int.repr (nested_field_offset2 t_struct_hmac_ctx_st [_key]))
+                 (Vptr cb cofs)));
+            `(field_at Tsh t_struct_hmac_ctx_st [_o_ctx] emptySha (Vptr cb cofs));
+            `(field_at Tsh t_struct_hmac_ctx_st [_i_ctx] emptySha (Vptr cb cofs));
+            `(field_at Tsh t_struct_hmac_ctx_st [_md_ctx] emptySha (Vptr cb cofs));
+            `(array_at tuchar Tsh IPADcont 0 i (Vptr pb pofs));
+            `(array_at tuchar Tsh DEFAULTcont i 64 (Vptr pb pofs));
+            `(array_at tuchar Tsh (ZnthV tuchar (map Vint (map Int.repr key))) 0
+                (Zlength key) (Vptr kb kofs)); `(K_vector KV)])
+          (n:=6%nat)
+          (v2:=(ZnthV tuchar (map Vint(map Int.repr (HMAC_FUN.mkArgZ (map Byte.repr (HMAC_FUN.mkKey key)) Ipad))) i)).
+          simpl; try reflexivity.
+          simpl; try reflexivity.
+          simpl; try reflexivity.
+          simpl; try reflexivity.
+          simpl; try reflexivity.
+          Focus 2. simpl. unfold value, nested_field_type2, t_struct_hmac_ctx_st; simpl.
+            reflexivity.
+          2: trivial.
+          repeat apply andp_right; rel_expr.
+            simpl. intros. unfold tarray. entailer. admit. (*TODO: relexpr in loopbody*)     
+          instantiate (1:=i). simpl. intros. normalize.
+           eapply rel_expr_tempvar.
+           admit. (*TODO: loadstoreSC*)
+          
+          admit. (*relexpr*)
+          unfold tuchar; simpl. apply ZnthV_map_Vint_is_int.
+            rewrite Zlength_correct. rewrite Zlength_correct in ZLI. rewrite map_length, ZLI. assumption.
+          red. omega.
+        }
+        { entailer. cancel.
+          rewrite (split_array_at (i+1) tuchar Tsh _ i 64); try omega. cancel.
+          unfold_data_at 2%nat. cancel.
+          rewrite (field_at_data_at Tsh t_struct_hmac_ctx_st [_key]); try reflexivity.
+          entailer.
+          rewrite at_offset'_eq.
+          2: simpl; rewrite Int.add_zero; reflexivity. unfold offset_val. cancel.
+          apply sepcon_derives.
+            rewrite (split_array_at i tuchar Tsh _ 0 (i+1)); try omega.
+            cancel.
+            apply array_lemmas.array_at_ext'.
+            unfold cVint, ZnthV; simpl; intros.
+            assert (i0=i). omega. subst i0. simpl.
+            destruct (zlt i 0). omega. simpl. rewrite upd_eq.
+            destruct (nth_mapVintZ i 
+             (HMAC_FUN.mkArgZ (map Byte.repr (HMAC_FUN.mkKey key)) Ipad)) as [n Hn].
+             rewrite ZLI; assumption.
+            rewrite Hn. unfold HMAC_FUN.mkArgZ in Hn; rewrite Hn. trivial.
+          apply array_lemmas.array_at_ext'.
+            unfold cVint, ZnthV; simpl; intros. rewrite upd_neq; trivial. omega.
+        } 
+      }
+    }
+
+    (*continuation after ipad-loop*)   
+    unfold_data_at 1%nat. normalize.
+    rewrite (field_at_data_at Tsh t_struct_hmac_ctx_st [_i_ctx]); try reflexivity. normalize.
+    rewrite at_offset'_eq.
+    2: simpl; rewrite Int.add_zero; reflexivity.
+    eapply semax_seq'.
+    frame_SEP 3.
+    forward_call (Vptr cb (Int.add cofs (Int.repr 108))).
+    { assert (FR: Frame = nil).
+        subst Frame. reflexivity.
+      rewrite FR. clear FR Frame. 
+      entailer. 
+    }
+    after_call. simpl. normalize. 
+
+    eapply semax_seq'.
+    frame_SEP 0 5 7.
+    remember (init_s256abs, 
+            HMAC_FUN.mkArgZ (map Byte.repr (HMAC_FUN.mkKey key)) Ipad,
+            Vptr cb (Int.add cofs (Int.repr 108)),
+            Vptr pb pofs, Tsh, 64, KV) as WITNESS.
+    forward_call WITNESS.
+    { assert (FR: Frame = nil).
+        subst Frame. reflexivity.
+      rewrite FR. clear FR Frame. 
+      subst WITNESS. entailer.
+      unfold data_block. rewrite ZLI. cancel.
+      entailer.
+      apply andp_right. 
+        simpl. apply prop_right. apply isbyte_map_ByteUnsigned.
+      apply array_lemmas.array_at_ext'.
+      unfold tuchars, cVint, ZnthV; simpl. intros. if_tac. omega. simpl. 
+      destruct (nth_mapVintZ i 
+           (HMAC_FUN.mkArgZ (map Byte.repr (HMAC_FUN.mkKey key)) Ipad)) as [n Hn].
+        rewrite ZLI; assumption.
+      rewrite Hn. unfold HMAC_FUN.mkArgZ in Hn; rewrite Hn. trivial.
+    }
+    after_call. simpl. intros rho. subst WITNESS. rewrite firstn_precise. normalize.
+      unfold HMAC_FUN.mkArgZ, HMAC_FUN.mkArg. repeat rewrite map_length.
+      unfold sixtyfour. rewrite combine_length, map_length, length_Nlist, HMAC_FUN.mkKey_length.
+      unfold SHA256_BlockSize; simpl. trivial.
+
+    simpl.
+    apply semax_pre with (P':=EX x : s256abs,
+     (PROP  ()
+     LOCAL  (tc_environ Delta; tc_environ Delta;
+       `(typed_true tint) (eval_id _reset);
+       `(eq (Vint (Int.repr 1))) (eval_id _reset);
+       `(eq (Vptr pb pofs)) (eval_var _pad (Tarray tuchar 64 noattr));
+       `(eq (Vptr cb cofs)) (eval_id _ctx); `(eq (Vptr kb kofs)) (eval_id _key);
+       `(eq (Vint (Int.repr l))) (eval_id _len);
+   (*`(eq KV) (eval_var sha._K256 (tarray tuint 64))*)
+        (fun rho => (eq KV) (eval_var sha._K256 (tarray tuint 64) (globals_only rho))))
+     SEP 
+      (`(fun a : environ =>
+      (PROP 
+       (update_abs
+          (HMAC_FUN.mkArgZ (map Byte.repr (HMAC_FUN.mkKey key)) Ipad)
+          init_s256abs x)
+       LOCAL ()
+       SEP  (`(K_vector KV);
+       `(sha256state_ x (Vptr cb (Int.add cofs (Int.repr 108))));
+       `(data_block Tsh
+           (HMAC_FUN.mkArgZ (map Byte.repr (HMAC_FUN.mkKey key)) Ipad)
+           (Vptr pb pofs)))) a) globals_only;
+      `(field_at Tsh t_struct_hmac_ctx_st [_key_length]
+          (if zlt 64 (Zlength key)
+           then Vint (Int.repr 32)
+           else Vint (Int.repr (Zlength key))) (Vptr cb cofs));
+      `(field_at Tsh t_struct_hmac_ctx_st [_key]
+          (map Vint (map Int.repr (HMAC_FUN.mkKey key))) (Vptr cb cofs));
+      `(field_at Tsh t_struct_hmac_ctx_st [_o_ctx] emptySha (Vptr cb cofs));
+      `(field_at Tsh t_struct_hmac_ctx_st [_md_ctx] emptySha (Vptr cb cofs));
+      `(array_at tuchar Tsh (tuchars (map Int.repr key)) 0 (Zlength key)
+         (Vptr kb kofs))))).
+    entailer. rename x0 into a. eapply exp_right with (x0:=a). entailer.
+    apply extract_exists_pre. intros ipadSHAabs.
+    rename H into SCc.
+    rename H0 into ACc.
+    normalize. simpl. normalize. rename H into ipadAbs_def.
+    rewrite (field_at_data_at Tsh t_struct_hmac_ctx_st [_o_ctx]); try reflexivity.
+    normalize.
+    rewrite at_offset'_eq.
+    2: simpl; rewrite Int.add_zero; reflexivity. unfold offset_val; simpl.
+
+    (*essentially the same for opad*)
+    forward_seq.
+    instantiate (1:= 
+  (PROP  ()
+   LOCAL  (tc_environ Delta; tc_environ Delta;
+   `(typed_true tint) (eval_id _reset);
+   `(eq (Vint (Int.repr 1))) (eval_id _reset);
+   `(eq (Vptr pb pofs)) (eval_var _pad (Tarray tuchar 64 noattr));
+   `(eq (Vptr cb cofs)) (eval_id _ctx); `(eq (Vptr kb kofs)) (eval_id _key);
+   `(eq (Vint (Int.repr l))) (eval_id _len);
+   (*`(eq KV) (eval_var sha._K256 (tarray tuint 64))*)
+     (fun rho => (eq KV) (eval_var sha._K256 (tarray tuint 64) (globals_only rho))))
+   SEP  (`(K_vector KV);
+   `(sha256state_ ipadSHAabs (Vptr cb (Int.add cofs (Int.repr 108))));
+   `(data_block Tsh
+       (HMAC_FUN.mkArgZ (map Byte.repr (HMAC_FUN.mkKey key)) Opad)
+       (Vptr pb pofs));
+   `(field_at Tsh t_struct_hmac_ctx_st [_key_length]
+       (if zlt 64 (Zlength key)
+        then Vint (Int.repr 32)
+        else Vint (Int.repr (Zlength key))) (Vptr cb cofs));
+   `(field_at Tsh t_struct_hmac_ctx_st [_key]
+       (map Vint (map Int.repr (HMAC_FUN.mkKey key))) (Vptr cb cofs));
+   `(data_at Tsh (nested_field_type2 t_struct_hmac_ctx_st [_o_ctx]) emptySha
+       (Vptr cb
+          (Int.add cofs
+             (Int.repr (nested_field_offset2 t_struct_hmac_ctx_st [_o_ctx])))));
+   `(field_at Tsh t_struct_hmac_ctx_st [_md_ctx] emptySha (Vptr cb cofs));
+   `(array_at tuchar Tsh (tuchars (map Int.repr key)) 0 (Zlength key)
+       (Vptr kb kofs))))). 
+    { (*opad loop*)
+      forward_for_simple_bound' 64 (EX i:Z, 
+  (PROP  ()
+   LOCAL  (`(typed_true (typeof (Etempvar _reset tint)))
+                     (eval_expr (Etempvar _reset tint));
+                 `(eq (Vint (Int.repr 1))) (eval_id _reset);
+                 `(eq (Vptr pb pofs)) (eval_var _pad (tarray tuchar 64));
+                 `(eq (Vptr cb cofs)) (eval_id _ctx);
+                 `(eq (Vptr kb kofs)) (eval_id _key);
+                 `(eq (Vint (Int.repr l))) (eval_id _len);
+   (*`(eq KV) (eval_var sha._K256 (tarray tuint 64))*)
+                 (fun rho => (eq KV) (eval_var sha._K256 (tarray tuint 64) (globals_only rho))))
+   SEP  (`(K_vector KV);
+   `(sha256state_ ipadSHAabs (Vptr cb (Int.add cofs (Int.repr 108))));
+   `(array_at tuchar Tsh OPADcont 0 i (Vptr pb pofs));
+   `(array_at tuchar Tsh IPADcont i 64 (Vptr pb pofs));
+   `(field_at Tsh t_struct_hmac_ctx_st [_key_length]
+       (if zlt 64 (Zlength key)
+        then Vint (Int.repr 32)
+        else Vint (Int.repr (Zlength key))) (Vptr cb cofs));
+   `(field_at Tsh t_struct_hmac_ctx_st [_key]
+       (map Vint (map Int.repr (HMAC_FUN.mkKey key))) (Vptr cb cofs));
+   `(data_at Tsh (nested_field_type2 t_struct_hmac_ctx_st [_o_ctx]) emptySha
+       (Vptr cb
+          (Int.add cofs
+             (Int.repr (nested_field_offset2 t_struct_hmac_ctx_st [_o_ctx])))));
+   `(field_at Tsh t_struct_hmac_ctx_st [_md_ctx] emptySha (Vptr cb cofs));
+   `(array_at tuchar Tsh (tuchars (map Int.repr key)) 0 (Zlength key)
+       (Vptr kb kofs))))).
+      { admit. (*_K256 closed*) }
+      { (*precondition implies "invariant"*)
+        rewrite array_at_emp. unfold data_block. entailer.
+        apply andp_right.
+          unfold array_at. normalize. rewrite ZLI in *. destruct H7.  destruct H8.
+            simpl in *. apply prop_right. omega.
+        cancel. rewrite ZLI. 
+            apply array_lemmas.array_at_ext'. 
+            unfold tuchars, cVint, ZnthV; simpl. intros. destruct (zlt i 0). omega.
+            destruct (nth_mapVintZ i 
+             (HMAC_FUN.mkArgZ (map Byte.repr (HMAC_FUN.mkKey key)) Ipad)) as [n Hn].
+            rewrite ZLI. assumption.
+            rewrite Hn. unfold HMAC_FUN.mkArgZ in Hn; rewrite Hn. trivial.            
+      }
+      { unfold normal_ret_assert, data_block. simpl. intros rho. 
+        rewrite array_at_emp. entailer.
+        apply andp_right. apply prop_right. apply isbyte_map_ByteUnsigned.
+        cancel. unfold tuchars. rewrite ZLO.
+            apply array_lemmas.array_at_ext'. 
+            unfold tuchars, cVint, ZnthV; simpl. intros. destruct (zlt i 0). omega.
+            destruct (nth_mapVintZ i 
+             (HMAC_FUN.mkArgZ (map Byte.repr (HMAC_FUN.mkKey key)) Opad)) as [n Hn].
+            rewrite ZLO. assumption. rewrite Hn. unfold HMAC_FUN.mkArgZ in Hn; rewrite Hn. trivial.
+      }
+      { (*unfold_data_at 1%nat. normalize.*)
+        rewrite (field_at_data_at Tsh t_struct_hmac_ctx_st [_key]); try reflexivity.
+        normalize. rename H into I. 
+        rewrite at_offset'_eq.
+        2: simpl; rewrite Int.add_zero; reflexivity.
+        eapply semax_pre0; [ apply now_later | ].
+        eapply semax_post_flipped'.
+        { subst PostResetBranch.
+          eapply NEWsemax_loadstore_array
+          with (P:= nil)
+          (Q:= [`(eq (Vint (Int.repr i))) (eval_id _i);
+            `(eq (Vint (Int.repr 64))) (eval_expr (Econst_int (Int.repr 64) tint));
+            `(typed_true tint) (eval_expr (Etempvar _reset tint));
+            `(eq (Vint (Int.repr 1))) (eval_id _reset);
+            `(eq (Vptr pb pofs)) (eval_var _pad (tarray tuchar 64));
+            `(eq (Vptr cb cofs)) (eval_id _ctx);
+            `(eq (Vptr kb kofs)) (eval_id _key);
+            `(eq (Vint (Int.repr l))) (eval_id _len);
+(*            `(eq KV) (eval_var sha._K256 (tarray tuint 64))*)
+              (fun rho => (eq KV) (eval_var sha._K256 (tarray tuint 64) (globals_only rho)))])
+          (R:= [`(K_vector KV);
+     `(sha256state_ ipadSHAabs (Vptr cb (Int.add cofs (Int.repr 108))));
+     `(array_at tuchar Tsh OPADcont 0 i (Vptr pb pofs));
+     `(array_at tuchar Tsh IPADcont i 64 (Vptr pb pofs));
+     `(field_at Tsh t_struct_hmac_ctx_st [_key_length]
+         (if zlt 64 (Zlength key)
+          then Vint (Int.repr 32)
+          else Vint (Int.repr (Zlength key))) (Vptr cb cofs));
+     `(data_at Tsh (nested_field_type2 t_struct_hmac_ctx_st [_key])
+         (map Vint (map Int.repr (HMAC_FUN.mkKey key)))
+         (offset_val
+            (Int.repr (nested_field_offset2 t_struct_hmac_ctx_st [_key]))
+            (Vptr cb cofs)));
+     `(data_at Tsh (nested_field_type2 t_struct_hmac_ctx_st [_o_ctx])
+         emptySha
+         (Vptr cb
+            (Int.add cofs
+               (Int.repr (nested_field_offset2 t_struct_hmac_ctx_st [_o_ctx])))));
+     `(field_at Tsh t_struct_hmac_ctx_st [_md_ctx] emptySha (Vptr cb cofs));
+     `(array_at tuchar Tsh (tuchars (map Int.repr key)) 0 (Zlength key)
+         (Vptr kb kofs))])
+          (n:=3%nat)
+          (v2:=(ZnthV tuchar (map Vint(map Int.repr (HMAC_FUN.mkArgZ (map Byte.repr (HMAC_FUN.mkKey key)) Opad))) i)).
+          simpl; try reflexivity.
+          simpl; try reflexivity.
+          simpl; try reflexivity.
+          simpl; try reflexivity.
+          simpl; try reflexivity.
+          Focus 2. simpl. unfold value, nested_field_type2, t_struct_hmac_ctx_st; simpl.
+            reflexivity.
+          2: trivial.
+          repeat apply andp_right; rel_expr.
+            simpl. intros. unfold tarray. entailer. admit. (*TODO: relexpr in loopbody*)     
+          instantiate (1:=i). simpl. intros. normalize.
+           eapply rel_expr_tempvar. admit. (*TODO: loadstoreSC*)
+
+          simpl. intros rho. entailer. admit. (*TODO rel_expr.*) 
+
+          unfold tuchar; simpl. apply ZnthV_map_Vint_is_int.
+            specialize (Zlength_mkArgZ (map Byte.repr (HMAC_FUN.mkKey key)) Opad).
+            repeat rewrite Zlength_correct; repeat rewrite map_length.
+            intros. rewrite H, HMAC_FUN.mkKey_length. unfold SHA256_BlockSize; simpl. assumption.
+          red. omega.
+        }
+        { entailer. cancel.
+          rewrite (split_array_at (i+1) tuchar Tsh _ i 64); try omega. cancel.
+          unfold_data_at 1%nat. cancel.
+          rewrite (field_at_data_at Tsh t_struct_hmac_ctx_st [_key]); try reflexivity.
+          rewrite at_offset'_eq.
+            2: simpl; rewrite Int.add_zero; reflexivity. unfold offset_val.
+          unfold_data_at 1%nat. entailer. cancel.
+          apply sepcon_derives.
+            rewrite (split_array_at i tuchar Tsh _ 0 (i+1)); try omega.
+            cancel.
+            apply array_lemmas.array_at_ext'.
+            unfold cVint, ZnthV; simpl; intros.
+            assert (i0=i). omega. subst i0. simpl.
+            destruct (zlt i 0). omega. simpl. rewrite upd_eq.
+            destruct (nth_mapVintZ i 
+             (HMAC_FUN.mkArgZ (map Byte.repr (HMAC_FUN.mkKey key)) Opad)) as [n Hn].
+              rewrite ZLO; assumption.
+            rewrite Hn. unfold HMAC_FUN.mkArgZ in Hn; rewrite Hn. trivial.
+          apply array_lemmas.array_at_ext'.
+            unfold cVint, ZnthV; simpl; intros. rewrite upd_neq; trivial. omega.
+        } 
+      }
+    }
+
+    (*continuation after opad-loop*)   
+    (*unfold_data_at 1%nat.*) (*normalize.
+    rewrite (field_at_data_at Tsh t_struct_hmac_ctx_st [_o_ctx]); try reflexivity. normalize.
+    rewrite at_offset'_eq.
+    2: simpl; rewrite Int.add_zero; reflexivity.*)
+    eapply semax_seq'.
+    frame_SEP 5.
+    forward_call (Vptr cb (Int.add cofs (Int.repr 216))).
+    { assert (FR: Frame = nil).
+        subst Frame. reflexivity.
+      rewrite FR. clear FR Frame. 
+      entailer. 
+    }
+    after_call. simpl. normalize.
+
+    unfold MORE_COMMANDS, abbreviate. (*WHY IS THIS NOT DONE AUTOMATICALLY?*)
+(*    make_sequential.
+    frame_SEP 0 1 3.*)
+    remember (init_s256abs, 
+            HMAC_FUN.mkArgZ (map Byte.repr (HMAC_FUN.mkKey key)) Opad,
+            Vptr cb (Int.add cofs (Int.repr 216)),
+            Vptr pb pofs, Tsh, 64, KV) as WITNESS.
+    forward_call WITNESS.
+    { assert (FR: Frame = [
+         `(sha256state_ ipadSHAabs (Vptr cb (Int.add cofs (Int.repr 108))));
+         `(field_at Tsh t_struct_hmac_ctx_st [_key_length]
+              (if zlt 64 (Zlength key)
+               then Vint (Int.repr 32)
+               else Vint (Int.repr (Zlength key))) (Vptr cb cofs));
+         `(field_at Tsh t_struct_hmac_ctx_st [_key]
+              (map Vint (map Int.repr (HMAC_FUN.mkKey key))) (Vptr cb cofs));
+         `(field_at Tsh t_struct_hmac_ctx_st [_md_ctx] emptySha (Vptr cb cofs));
+         `(array_at tuchar Tsh (tuchars (map Int.repr key)) 0 (Zlength key)
+              (Vptr kb kofs))]). 
+        subst Frame. reflexivity.
+      rewrite FR. clear FR Frame. 
+      subst WITNESS. entailer. cancel.
+    }
+    after_call. simpl. intros rho. subst WITNESS PostResetBranch.
+        rewrite firstn_precise. entailer.
+        rename x into x'.
+        rename x0 into opadSHAabs.
+        unfold sha256state_; normalize. rename r into iUpd. rename x into oUpd.
+        apply exp_right with (x:=ipadSHAabs). entailer.
+        apply exp_right with (x:=iUpd). entailer.
+        apply exp_right with (x:=opadSHAabs). entailer.
+        apply exp_right with (x:=oUpd). entailer.
+        unfold data_block.  rewrite ZLO. entailer. cancel.
+        unfold_data_at 3%nat. cancel.
+    rewrite (field_at_data_at Tsh t_struct_hmac_ctx_st [_i_ctx]); try reflexivity.
+    entailer.
+    rewrite at_offset'_eq.
+    2: simpl; rewrite Int.add_zero; reflexivity. unfold offset_val; simpl.
+
+    rewrite (field_at_data_at Tsh t_struct_hmac_ctx_st [_o_ctx]); try reflexivity.
+    entailer.
+    rewrite at_offset'_eq.
+    2: simpl; rewrite Int.add_zero; reflexivity. unfold offset_val; simpl.
+
+    cancel.
+
+      unfold HMAC_FUN.mkArgZ, HMAC_FUN.mkArg. repeat rewrite map_length.
+      unfold sixtyfour. rewrite combine_length, map_length, length_Nlist, HMAC_FUN.mkKey_length.
+      unfold SHA256_BlockSize; simpl. trivial.
+  }
+  { (*ELSE*) 
+    forward. entailer.
+  }
+}
+{ (*Continuation after if (reset*)
+  subst PostResetBranch. 
+  normalize.
+  apply extract_exists_pre; intros iSA. 
+  apply extract_exists_pre; intros iS. 
+  apply extract_exists_pre; intros oSA. 
+  apply extract_exists_pre; intros oS.
+  normalize. 
+  rename H into INNER. rename H0 into InnerRelate.
+  rename H1 into OUTER. rename H2 into OuterRelate.
+  unfold_data_at 1%nat.
+  (* eapply semax_seq'.
+  frame_SEP 3 4.*)
+   rewrite (field_at_data_at Tsh t_struct_hmac_ctx_st [_md_ctx]); try reflexivity.
+   normalize.
+   rename H into SCc. rename H0 into ACc.
+   rewrite at_offset'_eq.
+     2: simpl; rewrite Int.add_zero; reflexivity.
+   eapply semax_pre with (P':=PROP  ()
+     LOCAL  (`(eq pad) (eval_var _pad (tarray tuchar 64));
+       `(eq (Vptr cb cofs)) (eval_id _ctx); `(eq (Vptr kb kofs)) (eval_id _key);
+       `(eq (Vint (Int.repr l))) (eval_id _len);
+   (*`(eq KV) (eval_var sha._K256 (tarray tuint 64))*)
+     (fun rho => (eq KV) (eval_var sha._K256 (tarray tuint 64) (globals_only rho))))
+     SEP  (`(field_at Tsh t_struct_hmac_ctx_st [_key_length]
+            (if zlt 64 (Zlength key)
+            then Vint (Int.repr 32)
+            else Vint (Int.repr (Zlength key))) (Vptr cb cofs));
+          `(field_at Tsh t_struct_hmac_ctx_st [_o_ctx] oS (Vptr cb cofs));
+          `(field_at Tsh t_struct_hmac_ctx_st [_key]
+              (map Vint (map Int.repr (HMAC_FUN.mkKey key))) (Vptr cb cofs));
+          `(field_at Tsh t_struct_hmac_ctx_st [_i_ctx] iS (Vptr cb cofs));
+          `(data_at_ Tsh (tarray tuchar 64) pad);
+          `(array_at tuchar Tsh (tuchars (map Int.repr key)) 0 (Zlength key)
+              (Vptr kb kofs));
+          `(K_vector KV);
+          `(memory_block Tsh (Int.repr (sizeof (nested_field_type2 t_struct_hmac_ctx_st [_md_ctx])))
+             (offset_val
+                (Int.repr (nested_field_offset2 t_struct_hmac_ctx_st [_md_ctx]))
+             (Vptr cb cofs))))).
+     entailer. cancel.
+     unfold tarray. erewrite data_at__array_at_. 2: omega. 2: reflexivity. 
+     cancel.
+     eapply derives_trans.
+       apply data_at_data_at_. reflexivity. 
+       rewrite <- memory_block_data_at_; try reflexivity. entailer.
+
+  rewrite (field_at_data_at Tsh t_struct_hmac_ctx_st [_i_ctx]); try reflexivity.
+  normalize. 
+  rewrite at_offset'_eq.
+    2: simpl; rewrite Int.add_zero; reflexivity.
+
+  remember ((Tsh, Tsh),
+             Vptr cb cofs,
+             offset_val
+              (Int.repr (nested_field_offset2 t_struct_hmac_ctx_st [_i_ctx]))
+              (Vptr cb cofs),
+             mkTrep t_struct_SHA256state_st iS) as  WITNESS.
+  forward_call WITNESS.
+  { assert (FR: Frame = [
+     `(field_at Tsh t_struct_hmac_ctx_st [_key_length]
+        (if zlt 64 (Zlength key)
+         then Vint (Int.repr 32)
+         else Vint (Int.repr (Zlength key))) (Vptr cb cofs));
+     `(field_at Tsh t_struct_hmac_ctx_st [_o_ctx] oS (Vptr cb cofs));
+     `(field_at Tsh t_struct_hmac_ctx_st [_key]
+        (map Vint (map Int.repr (HMAC_FUN.mkKey key))) (Vptr cb cofs));
+     `(data_at_ Tsh (tarray tuchar 64) pad);
+     `(array_at tuchar Tsh (tuchars (map Int.repr key)) 0 (Zlength key)
+        (Vptr kb kofs)); `(K_vector KV)]).
+       subst Frame. reflexivity.
+    rewrite FR. clear FR Frame. 
+    subst WITNESS. entailer. cancel. 
+  }
+  after_call. subst WITNESS. normalize.  subst retval0. simpl. 
+
+  forward. (*return*)
+
+  remember (Int.unsigned (Int.repr (if zlt 64 (Zlength key) then 32 else Zlength key)))as KL.
+  rename x into x'.
+  apply exp_right with (x:=HMACabs iSA iSA oSA KL key). (*(HMAC_FUN.mkKey key)).*)
+  entailer.
+  apply andp_right. 
+    apply prop_right. unfold hmacInit. exists iSA, oSA.
+    rewrite Int.unsigned_repr. auto.
+    rewrite int_max_signed_eq  in KL2. rewrite int_max_unsigned_eq.
+     destruct (zlt 64 (Zlength key)); omega.    
+  unfold data_block. simpl_stackframe_of. entailer. cancel.
+  unfold hmacstate_, hmac_relate.
+  remember (if zlt 64 (Zlength key) then Vint (Int.repr 32)
+            else Vint (Int.repr (Zlength key))) as kl.
+
+  apply exp_right with
+    (x:=(iS, (iS, (oS, (kl, map Vint (map Int.repr (HMAC_FUN.mkKey key))))))).
+  simpl. entailer.
+  apply andp_right. apply prop_right.
+    split.
+      rewrite (updAbs_len _ _ _ INNER), Zlength_mkArgZ,
+           map_length, HMAC_FUN.mkKey_length; reflexivity.
+    split.
+      rewrite (updAbs_len _ _ _ OUTER), Zlength_mkArgZ,
+           map_length, HMAC_FUN.mkKey_length; reflexivity.
+    exists (Int.repr (if zlt 64 (Zlength key) then 32 else Zlength key)).
+    rewrite Int.unsigned_repr. 
+     split. destruct (zlt 64 (Zlength key)); trivial.
+     split; trivial.
+    rewrite int_max_signed_eq  in KL2. rewrite int_max_unsigned_eq.
+     destruct (zlt 64 (Zlength key)); omega.
+
+  unfold_data_at 3%nat. cancel.
+  rewrite (field_at_data_at Tsh t_struct_hmac_ctx_st [_i_ctx]); try reflexivity.
+  rewrite (field_at_data_at Tsh t_struct_hmac_ctx_st [_md_ctx]); try reflexivity.
+  entailer.
+}
+Qed.
